theories/Compositional_Structures/Basic_Modules/Component_Types/Social_Choice_Types/Ballot_Refinement.thy
@@ -1,3 +1,13 @@
+(*  File:       Ballot_Refinement.thy
+    Copyright   2022  Karlsruhe Institute of Technology (KIT)
+*)
+\<^marker>\<open>creator "Valentin Springsklee, Karlsruhe Institute of Technology (KIT)"\<close>
+
+chapter \<open>Data Refinement for Ranking\<close>
+
+section \<open>Preference Relation\<close>
+
+
 theory Ballot_Refinement
   imports Verified_Voting_Rule_Construction.Preference_Relation
   Verified_Voting_Rule_Construction.Preference_List
@@ -9,32 +19,16 @@ theory Ballot_Refinement
 
 begin
 
+subsection \<open>Refinement Relation for Ballots\<close>
 
-definition finite_set_rel where alt_set_rel_def_internal:
-  "finite_set_rel R \<equiv> (\<langle>R\<rangle>set_rel O br (\<lambda>x. x) (\<lambda> x. finite x))"
-
-
-lemma finite_set_rel_def[refine_rel_defs]: 
-  "\<langle>R\<rangle>finite_set_rel \<equiv> (\<langle>R\<rangle>set_rel O br (\<lambda>x. x) (\<lambda> x. finite x))"
-  by (simp add: alt_set_rel_def_internal relAPP_def)
-
-definition alt_set_rel_fixed :: "('a \<times> 'a) set \<Rightarrow> 'a set \<Rightarrow> ('a set \<times> 'a set) set"
-  where alt_set_rel_fixed_internal_def:
-  "alt_set_rel_fixed R A \<equiv> \<langle>R\<rangle>set_rel O br (\<lambda>x. x) (\<lambda>x. x = A) "
-
-lemma finite_alts:
-  assumes "(a, a') \<in> \<langle>R\<rangle>finite_set_rel" and "single_valued R" and "IS_LEFT_UNIQUE R"
-  shows "finite a" using assms  finite_set_rel_def in_br_conv
-  by (metis (no_types, lifting) IS_LEFT_UNIQUE_def Pair_inject finite_set_rel_transfer_back relcompE)
-
-lemma id_same_alts:
-  assumes "(A, A') \<in> \<langle>Id\<rangle>finite_set_rel"
-  shows "A' = A"
-  using assms  in_br_conv set_rel_id Id_O_R unfolding finite_set_rel_def
-  by (metis (no_types, lifting))
   
-abbreviation "ballot_rel \<equiv> br (pl_\<alpha>) (well_formed_pl)"
-            
+definition ballot_rel_def [refine_rel_defs]:
+  "ballot_rel \<equiv> br (pl_\<alpha>) (well_formed_pl)"
+
+lemma sv_bal_rel: "single_valued ballot_rel"
+  unfolding ballot_rel_def
+  by (simp)
+
 lemma linearorder_ref: 
   "(linear_order_on_l, linear_order_on) \<in> \<langle>Id\<rangle>set_rel \<rightarrow> ballot_rel \<rightarrow> bool_rel"                                 
 proof (refine_vcg, clarsimp_all)
@@ -42,7 +36,8 @@ proof (refine_vcg, clarsimp_all)
   fix bal:: "'a Preference_List" and bar:: "'a Preference_Relation"
   assume "(bal, bar) \<in> ballot_rel"
   from this show " linear_order_on_l alts bal = linear_order_on alts bar"
-  using in_br_conv linorder_l_imp_rel linorder_rel_imp_l
+    using in_br_conv linorder_l_imp_rel linorder_rel_imp_l
+    unfolding ballot_rel_def
     by metis
 qed
 
@@ -52,9 +47,8 @@ text \<open>We attempted to show a completeness lemma for our refinement of line
       not empty.\<close>
 
 lemma simple_list_abstraction_sketch:
-  shows "([1::nat,2], {(2::nat,1::nat), (2::nat,2::nat)
-, (1::nat,1::nat)}) \<in> ballot_rel"
-  unfolding in_br_conv well_formed_pl_def pl_\<alpha>_def
+  shows "([1::nat,2], {(2::nat,1::nat), (2::nat,2::nat), (1::nat,1::nat)}) \<in> ballot_rel"
+  unfolding in_br_conv well_formed_pl_def ballot_rel_def pl_\<alpha>_def 
   is_less_preferred_than_l.simps by auto
 
 
@@ -66,11 +60,13 @@ lemma ballot_prop_rel:
   shows "(l,r) \<in> ballot_rel"
   using assms by (metis in_br_conv relcompEpair)
 
+subsection \<open>Refinement Relation for Basic Operations\<close>
+
 lemma aboveref:                                          
   shows "(above_l, above) \<in> ballot_rel \<rightarrow> Id \<rightarrow> \<langle>Id\<rangle>list_set_rel"
   apply (refine_vcg)                                    
   unfolding list_set_rel_def
-  apply (auto) using aboveeq unfolding well_formed_pl_def in_br_conv above_l_def
+  apply (auto) using aboveeq unfolding well_formed_pl_def in_br_conv above_l_def ballot_rel_def
   by (metis distinct_take)
   
 lemma rankref: 
@@ -86,28 +82,14 @@ lemma is_less_preferred_than_ref:
   apply (refine_vcg)
   by (auto simp only: refine_rel_defs is_less_preferred_than_eq)
 
+subsection \<open>Refinement Relation for Profile\<close>
 
-abbreviation "profile_rel \<equiv> \<langle>ballot_rel\<rangle>list_rel"
+abbreviation  "profile_rel \<equiv> \<langle>ballot_rel\<rangle>list_rel"
 abbreviation "profile_on_A_rel A \<equiv> \<langle>ballot_on_A_rel A\<rangle>list_rel"
 
-term fun_rel
-
-term "{ (f,f'). \<forall>(a,a')\<in>A. (f a, f' a')\<in>B }"
-
-definition alt_and_profile_rel ::
-  "('a \<times> 'a) set \<Rightarrow> (('a set \<times> 'a list list) \<times> 'a set \<times> ('a \<times> 'a) set list) set"
-  where alt_and_profile_rel_def_internal: 
-"alt_and_profile_rel R \<equiv> 
-  {((A', pl),(A, pr)). (A', A) \<in> \<langle>R\<rangle>finite_set_rel
-    \<and> (pl, pr) \<in> profile_on_A_rel (A')}"
-
-lemma alt_and_profile_rel_def: 
-  "\<langle>R\<rangle>alt_and_profile_rel \<equiv> {((A', pl),(A, pr)). (A', A) \<in> \<langle>R\<rangle>finite_set_rel
-    \<and> (pl, pr) \<in> profile_on_A_rel (A')}"
-  by (simp add: alt_and_profile_rel_def_internal relAPP_def)
 
 lemma sv_prof_rel: "single_valued profile_rel"
-  by (simp add: list_rel_sv)
+  by (simp add: sv_bal_rel list_rel_sv)
 
 lemma profile_rel_imp_map_ballots:
   fixes pl :: "'a Profile_List"
@@ -116,8 +98,8 @@ lemma profile_rel_imp_map_ballots:
   shows "pr = map pl_\<alpha> pl"
 proof (-)
   from assms have "\<forall> i < length pl. (pl!i, pr!i) \<in> ballot_rel"
-    by (simp add: list_rel_pres_length param_nth)
-  from assms this show " pr = map pl_\<alpha> pl"
+    by (simp add:  list_rel_pres_length param_nth)
+  from assms this show " pr = map pl_\<alpha> pl" unfolding ballot_rel_def 
     by (metis in_br_conv  length_map list_rel_pres_length nth_equalityI nth_map) 
 qed
   
@@ -140,7 +122,7 @@ next
     from this have "(\<forall>i < length (fst x). (((fst x)!i), ((snd x)!i)) \<in> (ballot_rel))"
       using ballot_prop_rel
       by blast
-    from lrrel this show "x \<in> (profile_rel)"
+    from lrrel this show "x \<in> (profile_rel)" 
       by (metis list_rel_eq_listrel listrel_iff_nth prod.exhaust_sel relAPP_def)
   qed
 qed    
@@ -152,7 +134,7 @@ lemma profile_prop_list:
   assumes "(pl,pr) \<in> profile_on_A_rel A"
   shows "profile_l A pl"
   unfolding profile_l_def
-  using assms in_br_conv
+  using assms in_br_conv unfolding ballot_rel_def
   by (metis (full_types) list_rel_imp_same_length pair_in_Id_conv param_nth relcompEpair)
 
 lemma profile_ref:
@@ -163,9 +145,11 @@ lemma profile_ref:
   shows "profile_l A pl \<longleftrightarrow> profile A pr"
 proof (-)
   from prel have "\<forall>idx < length pl. ((pl!idx), (pr!idx)) \<in> ballot_rel"
-    using in_br_conv
+    using in_br_conv  unfolding  ballot_rel_def
     by (simp add: list_rel_pres_length param_nth)
-  from prel this show "profile_l A pl \<longleftrightarrow> profile A pr" using in_br_conv  profile_def profile_l_def
+  from prel this show "profile_l A pl \<longleftrightarrow> profile A pr" 
+    unfolding  ballot_rel_def
+     profile_def profile_l_def in_br_conv
     by (metis linorder_l_imp_rel linorder_rel_imp_l list_rel_pres_length)
 qed
 
@@ -179,20 +163,12 @@ proof (-)
   from assms have profrel: "(pl,pr) \<in> profile_rel"
     using profile_type_ref by metis
   from profl this show "profile A pr"
-    using profile_ref
+    using profile_ref  unfolding ballot_rel_def
     by (simp add: in_br_conv linorder_l_imp_rel list_rel_eq_listrel listrel_iff_nth 
         profile_def profile_l_def relAPP_def)
 qed
 
-
-abbreviation "ballot_impl_assn  R \<equiv> (arl_assn R)"
-
-abbreviation "profile_impl_assn  R \<equiv> (list_assn (ballot_impl_assn  R))"
-
-abbreviation "alts_set_impl_assn  R \<equiv> (hs.assn R)"
-
-abbreviation "result_impl_assn  R \<equiv> alts_set_impl_assn  R \<times>\<^sub>a alts_set_impl_assn  R \<times>\<^sub>a alts_set_impl_assn  R"
-
+section \<open>Monadic Definition of Limiting a Single Ballot\<close>
 
 definition "limit_monadic_inv A ballot \<equiv> \<lambda> (i, nbal).
   nbal = limit_l A (take i ballot)"
@@ -215,6 +191,15 @@ definition  limit_monadic :: "'a::{default, hashable, heap} set
     RETURN (nbal)
   }"                          
 
+subsection \<open>Correctness\<close>
+
+lemma limit_l_sound:
+  fixes A :: "'a set"
+  fixes bal :: "'a Preference_List"
+  assumes "well_formed_pl bal"
+  shows "well_formed_pl (limit_l A bal)"
+  using assms unfolding well_formed_pl_def
+  by auto
 
 
 lemma limit_monadic_refine:
@@ -228,16 +213,6 @@ lemma limit_monadic_refine:
   done
 
 
-lemma limit_l_sound:
-  fixes A :: "'a set"
-  fixes bal :: "'a Preference_List"
-  assumes "well_formed_pl bal"
-  shows "well_formed_pl (limit_l A bal)"
-  using assms unfolding well_formed_pl_def
-  by auto
-
-
-
 lemma limit_monadic_correct:
   shows "(uncurry limit_monadic, uncurry (RETURN oo limit))
       \<in> [\<lambda> (A, bal). finite A]\<^sub>f (\<langle>Id\<rangle>set_rel \<times>\<^sub>r ballot_rel) \<rightarrow> \<langle>ballot_rel\<rangle>nres_rel"
@@ -249,18 +224,32 @@ proof (intro frefI fun_relI nres_relI, auto simp del: limit.simps,
   assume balrel: "(bal, bar) \<in> ballot_rel"
   assume fina: "finite A"
   from balrel have wf: "well_formed_pl bal"
-   using in_br_conv
+   using in_br_conv  unfolding  ballot_rel_def
    by metis
-  from balrel have abs: "bar = pl_\<alpha> bal" unfolding in_br_conv by simp
+  from balrel have abs: "bar = pl_\<alpha> bal" unfolding   ballot_rel_def in_br_conv by simp
   from fina have refp: "(limit_monadic A bal \<le> SPEC(\<lambda> lim. lim = (limit_l A bal)))" 
       using limit_monadic_refine by blast
   from wf  have refb: "(limit_l A bal, limit A bar) \<in> ballot_rel" unfolding abs
-    unfolding in_br_conv  using limit_eq limit_l_sound by metis 
+    unfolding ballot_rel_def in_br_conv  using limit_eq limit_l_sound by blast
   from this have balref: "(SPEC (\<lambda>x. x = limit_l A bal)) \<le> \<Down> ballot_rel (SPEC (\<lambda>x. x = limit A bar))"
     by (metis (full_types) RETURN_SPEC_refine lhs_step_SPEC)
   show "limit_monadic A bal \<le> \<Down> ballot_rel (SPEC (\<lambda>x. x = limit A bar))"
     using  order_trans[OF refp balref] .
 qed
+
+subsection \<open>Separation Logic Assertions Relators for Eelectoral Module Data Type\<close>
+
+abbreviation "ballot_impl_assn  R \<equiv> (arl_assn R)"
+
+abbreviation "profile_impl_assn  R \<equiv> (list_assn (ballot_impl_assn R))"
+
+abbreviation "alts_set_impl_assn  R \<equiv> (hs.assn R)"
+
+abbreviation "result_impl_assn  R \<equiv> alts_set_impl_assn  R \<times>\<^sub>a alts_set_impl_assn  R \<times>\<^sub>a alts_set_impl_assn  R"
+
+subsection \<open>Imperative HOL Definition of Limit Function for Ballot\<close>
+
+text \<open>The old ballot remains valid on the heap. A new array list is created for the limited ballot.\<close>
 
 sepref_definition limit_sep is "uncurry limit_monadic" ::
   "(hs.assn id_assn)\<^sup>k *\<^sub>a (ballot_impl_assn id_assn)\<^sup>k \<rightarrow>\<^sub>a (ballot_impl_assn id_assn)"
